Improved mergesort's implementation

MergeSort.v
@@ -86,21 +86,22 @@ Proof.
   assumption.
 Qed.
 
-Fact Permutation_fold_right A xss : forall ys ys',
-  Permutation ys ys' ->
-  Permutation (ys ++ fold_right (@app A) [] xss) (fold_right (@app A) ys' (rev (map (@rev A) xss))).
+Definition concat A := fold_right (@app A) [].
+
+Lemma concat_app A xs ys :
+  concat A (xs ++ ys) = concat _ xs ++ concat A ys.
 Proof.
-  induction xss; simpl in *; intros ? ? HPermutation.
-  - rewrite app_nil_r.
-    eauto.
-  - rewrite app_assoc.
-    rewrite fold_right_app.
-    simpl.
-    apply IHxss.
-    eapply Permutation_trans.
-    + apply Permutation_app_comm.
-    + apply Permutation_app; eauto.
-      apply Permutation_rev.
+  induction xs; simpl in *;
+    repeat rewrite <- app_assoc;
+    congruence.
+Qed.
+
+Lemma concat_rev A xs :
+  concat A (rev (map (@rev _) xs)) = rev (concat _ xs).
+Proof.
+  induction xs; simpl in *;
+    repeat ((rewrite concat_app || rewrite app_nil_r || rewrite rev_app_distr); simpl in *);
+    congruence.
 Qed.
 
 Module MergeSort.
@@ -115,13 +116,13 @@ Module MergeSort.
     Hypothesis leb_trans : Transitive leb.
     Hint Resolve leb_trans.
 
-    Definition merge :
+    Definition rev_merge :
       forall xs, StronglySorted leb xs ->
       forall ys, StronglySorted leb ys ->
       forall acc,
       { ws | exists zs, ws = rev zs ++ acc /\ StronglySorted leb zs /\ Permutation zs (xs ++ ys) }.
     Proof.
-      refine (fix merge xs :=
+      refine (fix rev_merge xs :=
         match xs as xs0 return
           StronglySorted leb xs0 ->
           forall ys, StronglySorted leb ys ->
@@ -129,24 +130,26 @@ Module MergeSort.
           { ws | exists zs, ws = rev zs ++ acc
               /\ StronglySorted leb zs
               /\ Permutation zs (xs0 ++ ys) } with
-        | [] => fun _ ys _ acc => exist _ (rev_append ys acc) _
+        | [] => fun _ ys _ acc => exist _ (rev_append ys acc) (ex_intro _ ys _)
         | x :: xs' => fun _ =>
-            fix merge' ys :=
-              match ys with
-              | [] => fun _ acc => exist _ (rev_append xs' (x :: acc)) _
+            fix rev_merge' ys :=
+              match ys as ys0 return
+                StronglySorted leb ys0 ->
+                forall acc,
+                { ws | exists zs, ws = rev zs ++ acc
+                    /\ StronglySorted leb zs
+                    /\ Permutation zs (x :: xs' ++ ys0) }
+              with
+              | [] => fun _ acc => exist _ (rev_append xs' (x :: acc)) (ex_intro _ (x :: xs') _)
               | y :: ys' => fun _ acc => 
                   if Sumbool.sumbool_of_bool (leb x y) then
-                    let (zs, H) := merge xs' _ (y :: ys') _ (x :: acc) in
-                    exist _ zs _
+                    let (zs, H) := rev_merge xs' _ (y :: ys') _ (x :: acc) in
+                    exist _ zs (let (x0, _) := H in ex_intro _ (x :: x0) _)
                   else
-                    let (zs, _) := merge' ys' _ (y :: acc) in
-                    exist _ zs _
+                    let (zs, H) := rev_merge' ys' _ (y :: acc) in
+                    exist _ zs (let (x0, _) := H in ex_intro _ (y :: x0) _)
               end
-        end); try clear merge';
-        try match goal with
-        | H : exists _, _ |- _ => destruct H
-        end;
-        [ exists ys | exists (x :: xs') | | | exists (x :: x0) | | exists (y :: x0) ];
+        end); try clear rev_merge';
         repeat (simpl in *; match goal with
         | H : StronglySorted _ (_ :: _) |- _ => inversion H; clear H; subst
         | H : _ /\ _ |- _ => destruct H
@@ -155,6 +158,7 @@ Module MergeSort.
         | _ => rewrite <- app_assoc
         | _ => split
         | _ => apply SSorted_cons
+        | H : leb ?x ?y = false |- _ => destruct (leb_total x y); [ congruence | clear H ]
         end; subst);
         eauto;
         repeat match goal with
@@ -165,12 +169,11 @@ Module MergeSort.
         | |- Forall _ _ =>
             apply Forall_forall; intros
         end.
-      - apply (Permutation_in _ H0) in H3.
+      - apply (Permutation_in _ H1) in H3.
         apply in_app_iff in H3.
         destruct H3 as [| HIn]; eauto.
         inversion HIn; subst; eauto.
-      - destruct (leb_total x y); [ congruence |].
-        apply (Permutation_in _ H0) in H3.
+      - apply (Permutation_in _ H1) in H3.
         apply in_app_iff with (l := x :: xs') in H3.
         destruct H3 as [HIn |]; eauto.
         inversion HIn; subst; eauto.
@@ -183,66 +186,179 @@ Module MergeSort.
       forall acc,
       { zss | exists xss', zss = rev (map (@rev t) xss') ++ acc /\ length xss' = div2 (S (length xss))
           /\ Forall (StronglySorted leb) xss'
-          /\ Permutation (fold_right (@app _) [] xss') (fold_right (@app _) [] xss) }.
+          /\ Permutation (concat _ xss') (concat _ xss) }.
     Proof.
       refine (fix meld xss :=
-        match xss with
-        | [] => fun _ acc => exist _ acc _
-        | [xs] => fun _ acc => exist _ (rev xs :: acc) _
+        match xss as xss0 return
+          Forall (StronglySorted leb) xss0 ->
+          forall acc,
+          { zss | exists xss', zss = rev (map (@rev t) xss') ++ acc /\ length xss' = div2 (S (length xss0))
+              /\ Forall (StronglySorted leb) xss'
+              /\ Permutation (concat _ xss') (concat _ xss0) }
+        with
+        | [] => fun _ acc => exist _ acc (ex_intro _ [] _)
+        | [xs] => fun _ acc => exist _ (rev xs :: acc) (ex_intro _ [xs] _)
         | xs :: xs' :: xss' => fun _ acc =>
-            let (ys, _) := merge xs _ xs' _ [] in
-            let (yss, _) := meld xss' _ (ys :: acc) in
-            exist _ yss _
-        end); clear meld;
-        repeat match goal with
-        | H : exists _, _ |- _ => destruct H
-        end;
-        [ exists (@nil (list t)) | exists [xs] | | | | exists (x0 :: x) ];
+            let (ys, H1) := rev_merge xs _ xs' _ [] in
+            let (yss, H2) := meld xss' _ (ys :: acc) in
+            exist _ yss (let (zs, _) := H1 in let (zss, _) := H2 in ex_intro _ (zs :: zss) _)
+        end);
         repeat (simpl in *; match goal with
         | _ => rewrite app_nil_r in *
         | _ => rewrite rev_involutive in *
         | H : Forall _ (_ :: _) |- _ =>
             inversion H; clear H; subst
         | H : _ /\ _ |- _ => destruct H
+        | H : exists _, _ |- _ => destruct H
         | _ => rewrite <- app_assoc
         | _ => split
         end; subst); eauto.
       rewrite app_assoc.
       apply Permutation_app; eauto.
     Defined.
+
+    Definition incr : forall xs acc curr prev,
+      Forall (fun x => leb x prev) curr ->
+      StronglySorted (fun x y => leb y x) curr ->
+      Forall (StronglySorted leb) acc ->
+      { xss | Permutation (concat _ xss) (concat _ acc ++ prev :: curr ++ xs)
+          /\ Forall (StronglySorted leb) xss }.
+    Proof.
+      refine (fix incr xs :=
+        match xs as xs0 return
+          forall acc curr prev,
+          Forall (fun x => leb x prev) curr ->
+          StronglySorted (fun x y => leb y x) curr ->
+          Forall (StronglySorted leb) acc ->
+          { xss | Permutation (concat _ xss) (concat _ acc ++ prev :: curr ++ xs0)
+              /\ Forall (StronglySorted leb) xss }
+        with
+        | [] => fun acc curr prev _ _ _ => exist _ (rev_append curr [prev] :: acc) _
+        | x :: xs => fun acc curr prev _ _ _ =>
+            if Sumbool.sumbool_of_bool (leb prev x) then _
+            else _
+        end
+      with decr xs :=
+        match xs as xs0 return forall acc curr prev,
+          Forall (leb prev) curr ->
+          StronglySorted leb curr ->
+          Forall (StronglySorted leb) acc ->
+          { xss | Permutation (concat _ xss) (concat _ acc ++ prev :: curr ++ xs0)
+              /\ Forall (StronglySorted leb) xss } 
+        with
+        | [] => fun acc curr prev _ _ _ => exist _ ((prev :: curr) :: acc) _
+        | x :: xs => fun acc curr prev _ _ _ =>
+            if Sumbool.sumbool_of_bool (leb x prev) then _
+            else _
+        end
+      for incr);
+      [ 
+      | refine (let (zss, _) := incr xs0 acc (prev :: curr) x _ _ _ in exist _ zss _)
+      | refine (let (zss, _) := decr xs0 (rev curr :: acc) [prev] x _ _ _ in exist _ zss _)
+      | 
+      | refine (let (zss, _) := decr xs0 acc (prev :: curr) x _ _ _ in exist _ zss _)
+      | refine (let (zss, _) := incr xs0 (curr :: acc) [prev] x _ _ _ in exist _ zss _) ];
+      repeat (match goal with
+      | _ => rewrite app_nil_r
+      | _ => rewrite <- app_assoc in *
+      | _ => rewrite rev_append_rev in *
+      | _ => apply Forall_rev
+      | _ => apply StronglySorted_app
+      | _ => apply StronglySorted_rev
+      | H : _ /\ _ |- _ =>  destruct H
+      | H : exists _, _ |- _ => destruct H
+      | |- Forall _ (_ :: _) => constructor
+      | H : Forall _ ?l |- Forall _ ?l => eapply Forall_impl; [| apply H ]; intros
+      | H : leb ?x ?y = false |- _ => destruct (leb_total x y); [ congruence | clear H ]
+      | _ => split
+      end; subst; simpl in *);
+      eauto.
+      - etransitivity.
+        + apply Permutation_app_comm.
+        + etransitivity.
+          * apply Permutation_middle.
+          * apply Permutation_app_head.
+            apply Permutation_cons.
+            symmetry.
+            apply Permutation_rev.
+      - etransitivity; eauto.
+        apply Permutation_app_head.
+        apply Permutation_middle with (l1 := prev :: curr).
+      - etransitivity; eauto.
+        etransitivity.
+        + rewrite app_assoc.
+          apply Permutation_app.
+          * apply Permutation_app_comm.
+          * reflexivity.
+        + rewrite <- app_assoc.
+          apply Permutation_app_head.
+          symmetry.
+          etransitivity.
+          * apply Permutation_middle.
+          * { apply Permutation_app.
+              - apply Permutation_rev.
+              - eauto. }
+      - apply Permutation_app_comm with (l := prev :: curr).
+      - etransitivity; eauto.
+        apply Permutation_app_head.
+        apply Permutation_middle with (l1 := prev :: curr).
+      - etransitivity; eauto.
+        etransitivity.
+        + rewrite app_assoc.
+          apply Permutation_app.
+          * apply Permutation_app_comm.
+          * reflexivity.
+        + rewrite <- app_assoc.
+          apply Permutation_app_head.
+          symmetry.
+          etransitivity.
+          * apply Permutation_middle.
+          * apply Permutation_app_head.
+            eauto.
+    Defined.
   End Tools.
+
+  Arguments ltof A f a b /.
 
   Definition merge_sort (t : Set) (leb : t -> t -> bool)
     (leb_total : forall x y, leb x y \/ leb y x)
     (leb_trans : Transitive leb) xs :
     { xs' | StronglySorted leb xs' /\ Permutation xs' xs }.
   Proof.
-    refine (let (xs', _) := Fix
-        (well_founded_ltof _ (@length _))
-        (fun xss =>
-          forall is_rev : bool,
-          Forall (StronglySorted (if is_rev then fun x y => leb y x else leb)) xss ->
-          Permutation (fold_right (@app _) [] xss) xs ->
-          { xs' | StronglySorted leb xs' /\ Permutation xs' xs })
-        (fun xss =>
-          match xss with
-          | [] => fun _ _ _ _ => exist _ [] _
-          | [xs] => fun _ is_rev _ _ =>
-              if Sumbool.sumbool_of_bool is_rev then exist _ (rev xs) _
-              else exist _ xs _
-          | xs :: ys :: xss => fun iter_meld is_rev _ _ =>
-              if Sumbool.sumbool_of_bool is_rev then
-                let (xss', _) :=
-                  meld _ (fun x y => leb y x) _ _ (xs :: ys :: xss) _ [] in
-                  iter_meld xss' _ (negb is_rev) _ _
-              else
-                let (xss', _) := meld _ leb _ _ (xs :: ys :: xss) _ [] in
-                iter_meld xss' _ (negb is_rev) _ _
-          end)
-        (map (fun x => [x]) xs) false _ _ in
-      exist _ xs' _);
+    refine (match xs as xs0 return { xs' | StronglySorted leb xs' /\ Permutation xs' xs0 } with
+      | [] => exist _ [] _
+      | x :: xs =>
+          let (xss, _) := incr _ leb _ _ xs [] [] x _ _ _ in
+          let (xs', _) :=
+            Fix
+              (well_founded_ltof _ (@length _))
+              (fun xss =>
+                forall is_rev : bool,
+                Forall (StronglySorted (if is_rev then fun x y => leb y x else leb)) xss ->
+                Permutation (concat _ xss) (x :: xs) ->
+                { xs' | StronglySorted leb xs' /\ Permutation xs' (x :: xs) })
+              (fun xss =>
+                match xss with
+                | [] => fun _ _ _ _ => exist _ [] _
+                | [xs] => fun _ is_rev _ _ =>
+                    if Sumbool.sumbool_of_bool is_rev then exist _ (rev xs) _
+                    else exist _ xs _
+                | xs :: ys :: xss => fun iter_meld is_rev _ _ =>
+                    if Sumbool.sumbool_of_bool is_rev then
+                      let (xss', _) :=
+                        meld _ (fun x y => leb y x) _ _ (xs :: ys :: xss) _ [] in
+                        iter_meld xss' _ (negb is_rev) _ _
+                    else
+                      let (xss', _) := meld _ leb _ _ (xs :: ys :: xss) _ [] in
+                      iter_meld xss' _ (negb is_rev) _ _
+                end) xss false _ _ in
+          exist _ xs' _
+      end);
       repeat (simpl in *; match goal with
+      | _ => rewrite rev_length
+      | _ => rewrite map_length
       | _ => rewrite app_nil_r in *
+      | _ => rewrite concat_rev
       | _ => apply StronglySorted_rev
       | _ => apply Forall_rev
       | _ => apply Forall_map
@@ -253,53 +369,24 @@ Module MergeSort.
       | _ => split
       | H : context [if ?b then _ else _] |- _ => destruct b
       | H : Forall _ ?l |- Forall _ ?l => eapply Forall_impl; [| apply H ]
+      | |- Permutation (rev ?xs) _ =>
+          apply Permutation_trans with (l' := rev (rev xs));
+          [ apply Permutation_rev
+          | rewrite rev_involutive ]
       end; subst);
       eauto.
-    - eapply Permutation_trans.
-      + apply Permutation_rev.
-      + rewrite rev_involutive.
-        eauto.
-    - unfold ltof.
-      simpl in *.
-      rewrite rev_length.
-      rewrite map_length.
-      destruct (length xss0).
+    - destruct (length xss1).
       + omega.
-      + rewrite H.
+      + rewrite H2.
         apply le_n_S.
         apply lt_div2 with (n := S (S n)).
         omega.
-    - apply Permutation_sym.
-      eapply Permutation_trans.
-      + apply Permutation_sym.
-        eauto.
-      + eapply Permutation_trans.
-        * apply Permutation_sym.
-          eauto.
-        * apply Permutation_fold_right with (A := t) (ys := []).
-          eauto.
-    - unfold ltof.
-      simpl in *.
-      rewrite rev_length.
-      rewrite map_length.
-      destruct (length xss0).
+    - destruct (length xss1).
       + omega.
-      + rewrite H.
+      + rewrite H2.
         apply le_n_S.
         apply lt_div2 with (n := S (S n)).
         omega.
-    - apply Permutation_sym.
-      eapply Permutation_trans.
-      + apply Permutation_sym.
-        eauto.
-      + eapply Permutation_trans.
-        * apply Permutation_sym.
-          eauto.
-        * apply Permutation_fold_right with (A := t) (ys := []).
-          eauto.
-    - apply Forall_forall.
-      eauto.
-    - induction xs; simpl; eauto.
   Defined.
 End MergeSort.
 
@@ -310,9 +397,9 @@ Extract Constant map => "List.map".
 Extract Constant app => "( @ )".
 Extract Constant rev => "List.rev".
 Extract Constant rev_append => "List.rev_append".
-Extract Constant Sumbool.sumbool_of_bool => "(fun b => b)".
+Extract Constant Sumbool.sumbool_of_bool => "(fun b -> b)".
 Extract Constant negb => "not".
-Extraction (* "mergeSort.ml" *) MergeSort.
+Extraction "mergeSort.ml" MergeSort.
 
 (* FUCKIN' HEAVY COMPUTATION *)
 (* Eval compute in NatSort.merge_sort [1; 1; 4; 5; 1; 4]. *)
